Rewrote the data structures storing state and IO in a module to use a Tree instead of a bunch of flat lists
This simplifies everything! And allows for modular design now (and potentially modular reasoning later).

PrettyPrinter/ModPrinter.hs
@@ -27,91 +27,225 @@ ppKindDecl q k = ppIndent q ++ ppKindImmStart q k
 clog2 :: Integer -> Integer
 clog2 = ceiling . (logBase 2) . fromIntegral
 
-condMem :: Integer -> Kind -> Integer -> String -> String
-condMem n k p s = condPrint (n > 0 && size k > 0 && p > 0) s
+sizeElem :: ModElem -> Bool
+sizeElem (EReg r) = size (regKind r) > 0
+sizeElem (EMem m) = size (memKind m) > 0 && memSize m > 0 && memPort m > 0
+sizeElem (ESend k) = size k > 0
+sizeElem (ERecv k) = size k > 0
 
-ppIfc :: Int -> CompiledModule -> String
-ppIfc q ((Build_ModDecl regs mems regUs memUs sends recvs, tmps), compiled) =
-  concatMap (\(i, (s, (Build_Mem n k p _))) -> condMem n k p $ ppKindDecl q (Array p (Bit (clog2 n))) ++ ppMem "Rq" (s, i) ++ ";\n") (tag mems)
-  ++ concatMap (\(i, (s, (Build_Mem n k p _))) -> condMem n k p $ ppKindDecl q (Array p Bool) ++ ppMem "RqEn" (s, i) ++ ";\n") (tag mems)
-  ++ concatMap (\(i, (s, (Build_Mem n k p _))) -> condMem n k p $ ppKindDecl q (Bit (clog2 n)) ++ ppMem "WrIdx" (s, i) ++ ";\n") (tag mems)
-  ++ concatMap (\(i, (s, (Build_Mem n k p _))) -> condMem n k p $ ppKindDecl q k ++ ppMem "WrVal" (s, i) ++ ";\n") (tag mems)
-  ++ concatMap (\(i, (s, (Build_Mem n k p _))) -> condMem n k p $ ppKindDecl q Bool ++ ppMem "WrEn" (s, i) ++ ";\n") (tag mems)
-  ++ concatMap (\(i, (s, (Build_MemU n k p))) -> condMem n k p $ ppKindDecl q (Array p (Bit (clog2 n))) ++ ppMem "URq" (s, i) ++ ";\n") (tag memUs)
-  ++ concatMap (\(i, (s, (Build_MemU n k p))) -> condMem n k p $ ppKindDecl q (Array p Bool) ++ ppMem "URqEn" (s, i) ++ ";\n") (tag memUs)
-  ++ concatMap (\(i, (s, (Build_MemU n k p))) -> condMem n k p $ ppKindDecl q (Bit (clog2 n)) ++ ppMem "UWrIdx" (s, i) ++ ";\n") (tag memUs)
-  ++ concatMap (\(i, (s, (Build_MemU n k p))) -> condMem n k p $ ppKindDecl q k ++ ppMem "UWrVal" (s, i) ++ ";\n") (tag memUs)
-  ++ concatMap (\(i, (s, (Build_MemU n k p))) -> condMem n k p $ ppKindDecl q Bool ++ ppMem "UWrEn" (s, i) ++ ";\n") (tag memUs)
+dfsModElems :: Tree ModElem -> [([String], ModElem)]
+dfsModElems tree = helper [] tree
+  where
+    helper path (Leaf name elem) = [(name : path, elem)]
+    helper path (Node name children) =
+      concatMap (helper (name : path)) children
 
-ppMod :: CompiledModule -> String
-ppMod mod@((Build_ModDecl regs mems regUs memUs sends recvs, tmps), compiled) =
-  "module system (\n"
-  ++ concatMap (\(i, (s, k)) -> condPrint (size k > 0) $ ppIndent 1 ++ "output " ++ ppKindImmStart 1 k ++ "decl_" ++ ppMeth "Send" (s, i) ++ ",\n") (tag sends)
-  ++ concatMap (\(i, (s, k)) -> ppIndent 1 ++ "output " ++ ppKindImmStart 1 Bool ++ "decl_" ++ ppMeth "SendEn" (s, i) ++ ",\n") (tag sends)
-  ++ concatMap (\(i, (s, (Build_Mem n k p _))) -> condMem n k p $ ppIndent 1 ++ "output " ++ ppKindImmStart 1 (Array p (Bit (clog2 n))) ++ "decl_" ++ ppMem "Rq" (s, i) ++ ",\n") (tag mems)
-  ++ concatMap (\(i, (s, (Build_Mem n k p _))) -> condMem n k p $ ppIndent 1 ++ "output " ++ ppKindImmStart 1 (Array p Bool) ++ "decl_" ++ ppMem "RqEn" (s, i) ++ ",\n") (tag mems)
-  ++ concatMap (\(i, (s, (Build_Mem n k p _))) -> condMem n k p $ ppIndent 1 ++ "output " ++ ppKindImmStart 1 (Bit (clog2 n)) ++ "decl_" ++ ppMem "WrIdx" (s, i) ++ ",\n") (tag mems)
-  ++ concatMap (\(i, (s, (Build_Mem n k p _))) -> condMem n k p $ ppIndent 1 ++ "output " ++ ppKindImmStart 1 k ++ "decl_" ++ ppMem "WrVal" (s, i) ++ ",\n") (tag mems)
-  ++ concatMap (\(i, (s, (Build_Mem n k p _))) -> condMem n k p $ ppIndent 1 ++ "output " ++ ppKindImmStart 1 Bool ++ "decl_" ++ ppMem "WrEn" (s, i) ++ ",\n") (tag mems)
-  ++ concatMap (\(i, (s, (Build_MemU n k p))) -> condMem n k p $ ppIndent 1 ++ "output " ++ ppKindImmStart 1 (Array p (Bit (clog2 n))) ++ "decl_" ++ ppMem "URq" (s, i) ++ ",\n") (tag memUs)
-  ++ concatMap (\(i, (s, (Build_MemU n k p))) -> condMem n k p $ ppIndent 1 ++ "output " ++ ppKindImmStart 1 (Array p Bool) ++ "decl_" ++ ppMem "URqEn" (s, i) ++ ",\n") (tag memUs)
-  ++ concatMap (\(i, (s, (Build_MemU n k p))) -> condMem n k p $ ppIndent 1 ++ "output " ++ ppKindImmStart 1 (Bit (clog2 n)) ++ "decl_" ++ ppMem "UWrIdx" (s, i) ++ ",\n") (tag memUs)
-  ++ concatMap (\(i, (s, (Build_MemU n k p))) -> condMem n k p $ ppIndent 1 ++ "output " ++ ppKindImmStart 1 k ++ "decl_" ++ ppMem "UWrVal" (s, i) ++ ",\n") (tag memUs)
-  ++ concatMap (\(i, (s, (Build_MemU n k p))) -> condMem n k p $ ppIndent 1 ++ "output " ++ ppKindImmStart 1 Bool ++ "decl_" ++ ppMem "UWrEn" (s, i) ++ ",\n") (tag memUs)
-  ++ concatMap (\(i, (s, k)) -> condPrint (size k /= 0) $ ppIndent 1 ++ "input " ++ ppKindImmStart 1 k ++ " " ++ ppMeth "Recv" (s, i) ++ ",\n") (tag recvs)
-  ++ concatMap (\(i, (s, (Build_Mem n k p _))) -> condMem n k p $ ppIndent 1 ++ "input " ++ ppKindImmStart 1 (Array p k) ++ ppMem "Rp" (s, i) ++ ",\n") (tag mems)
-  ++ concatMap (\(i, (s, (Build_MemU n k p))) -> condMem n k p $ ppIndent 1 ++ "input " ++ ppKindImmStart 1 (Array p k) ++ ppMem "URp" (s, i) ++ ",\n") (tag memUs)
-  ++ ppIndent 1 ++ "input CLK,\n"
-  ++ ppIndent 1 ++ "input RESET);\n"
-  ++ concatMap (\(i, (s, k)) -> condPrint (size k /= 0) $ ppKindDecl 1 k ++ ppMeth "Send" (s, i) ++ ";\n") (tag sends)
-  ++ concatMap (\(i, (s, k)) -> ppKindDecl 1 Bool ++ ppMeth "SendEn" (s, i) ++ ";\n") (tag sends)
-  ++ ppIfc 1 mod
-  ++ concatMap (\(i, (s, (Build_Reg k _))) -> condPrint (size k /= 0) $ ppKindDecl 1 k ++ "decl_" ++ ppReg (s, i) ++ ";\n") (tag regs)
-  ++ concatMap (\(i, (s, k)) -> condPrint (size k /= 0) $ ppKindDecl 1 k ++ "decl_" ++ ppRegU (s, i) ++ ";\n") (tag regUs)
-  ++ concatMap (\(i, (s, (Build_Reg k _))) -> condPrint (size k /= 0) $ ppKindDecl 1 k ++ ppReg (s, i) ++ ";\n") (tag regs)
-  ++ concatMap (\(i, (s, k)) -> condPrint (size k /= 0) $ ppKindDecl 1 k ++ ppRegU (s, i) ++ ";\n") (tag regUs)
-  ++ concatMap (\(i, (s, k)) -> condPrint (size k /= 0) $ ppKindDecl 1 k ++ ppTmp (s, integerFromInt (Prelude.length tmps) - 1 - i) ++ ";\n") (tag tmps)
-  ++ ppIndent 1 ++ "initial begin\n"
-  ++ concatMap (\(i, (s, (Build_Reg k val))) -> condPrint (size k /= 0) $ ppIndent 2 ++ "decl_" ++ ppReg (s, i) ++ " = " ++ ppConst k val ++ ";\n") (tag regs)
-  ++ ppIndent 1 ++ "end\n"
-  ++ ppIndent 1 ++ "always_ff @(posedge CLK) begin\n"
-  ++ ppIndent 2 ++ "if(RESET) begin\n"
-  ++ concatMap (\(i, (s, (Build_Reg k val))) -> condPrint (size k /= 0) $ ppIndent 3 ++ "decl_" ++ ppReg (s, i) ++ " <= " ++ ppConst k val ++ ";\n") (tag regs)
-  ++ ppIndent 2 ++ "end else begin\n"
-  ++ concatMap (\(i, (s, (Build_Reg k _))) -> condPrint (size k /= 0) $ ppIndent 3 ++ "decl_" ++ ppReg (s, i) ++ " <= " ++ ppReg (s, i) ++ ";\n") (tag regs)
-  ++ concatMap (\(i, (s, k)) -> condPrint (size k /= 0) $ ppIndent 3 ++ "decl_" ++ ppRegU (s, i) ++ " <= " ++ ppRegU (s, i) ++ ";\n") (tag regUs)
-  ++ ppIndent 2 ++ "end\n"
-  ++ ppIndent 1 ++ "end\n"
-  ++ ppIndent 1 ++ "always_comb begin\n"
-  ++ concatMap (\(i, (s, (Build_Reg k _))) -> condPrint (size k /= 0) $ ppIndent 2 ++ ppReg (s, i) ++ " = decl_" ++ ppReg (s, i) ++ ";\n") (tag regs)
-  ++ concatMap (\(i, (s, k)) -> condPrint (size k /= 0) $ ppIndent 2 ++ ppRegU (s, i) ++ " = decl_" ++ ppRegU (s, i) ++ ";\n") (tag regUs)
-  ++ concatMap (\(i, (s, k)) -> condPrint (size k /= 0) $ ppIndent 2 ++ ppTmp (s, integerFromInt (Prelude.length tmps) - 1 - i) ++ " = " ++ show (size k) ++ "\'h0;\n") (tag tmps)
-  ++ concatMap (\(i, (s, k)) -> condPrint (size k /= 0) $ ppIndent 2 ++ ppMeth "Send" (s, i) ++ " = " ++ show (size k) ++ "\'h0;\n") (tag sends)
-  ++ concatMap (\(i, (s, k)) -> ppIndent 2 ++ ppMeth "SendEn" (s, i) ++ " = 1\'b0;\n") (tag sends)
-  ++ concatMap (\(i, (s, (Build_Mem n k p _))) -> condMem n k p $ ppIndent 2 ++ ppMem "Rq" (s, i) ++ " = " ++ show (p * clog2 n) ++ "\'h0;\n") (tag mems)
-  ++ concatMap (\(i, (s, (Build_Mem n k p _))) -> condMem n k p $ ppIndent 2 ++ ppMem "RqEn" (s, i) ++ " = " ++ show p ++ "\'h0;\n") (tag mems)
-  ++ concatMap (\(i, (s, (Build_Mem n k p _))) -> condMem n k p $ ppIndent 2 ++ ppMem "WrIdx" (s, i) ++ " = " ++ show (clog2 n) ++ "\'h0;\n") (tag mems)
-  ++ concatMap (\(i, (s, (Build_Mem n k p _))) -> condMem n k p $ ppIndent 2 ++ ppMem "WrVal" (s, i) ++ " = " ++ show (size k) ++ "\'h0;\n") (tag mems)
-  ++ concatMap (\(i, (s, (Build_Mem n k p _))) -> condMem n k p $ ppIndent 2 ++ ppMem "WrEn" (s, i) ++ " = " ++ "1\'h0;\n") (tag mems)
-  ++ concatMap (\(i, (s, (Build_MemU n k p))) -> condMem n k p $ ppIndent 2 ++ ppMem "URq" (s, i) ++ " = " ++ show (p * clog2 n) ++ "\'h0;\n") (tag memUs)
-  ++ concatMap (\(i, (s, (Build_MemU n k p))) -> condMem n k p $ ppIndent 2 ++ ppMem "URqEn" (s, i) ++ " = " ++ show p ++  "\'b0;\n") (tag memUs)
-  ++ concatMap (\(i, (s, (Build_MemU n k p))) -> condMem n k p $ ppIndent 2 ++ ppMem "UWrIdx" (s, i) ++ " = " ++ show (clog2 n) ++ "\'h0;\n") (tag memUs)
-  ++ concatMap (\(i, (s, (Build_MemU n k p))) -> condMem n k p $ ppIndent 2 ++ ppMem "UWrVal" (s, i) ++ " = " ++ show (size k) ++ "\'h0;\n") (tag memUs)
-  ++ concatMap (\(i, (s, (Build_MemU n k p))) -> condMem n k p $ ppIndent 2 ++ ppMem "UWrEn" (s, i) ++ " = " ++ "1\'b0;\n") (tag memUs)
-  ++ "\n"
-  ++ ppCompiled 2 compiled
-  ++ "\n"
-  ++ concatMap (\(i, (s, k)) -> condPrint (size k /= 0) $ ppIndent 2 ++ "decl_" ++ ppMeth "Send" (s, i) ++ " = " ++ ppMeth "Send" (s, i) ++ ";\n") (tag sends)
-  ++ concatMap (\(i, (s, k)) -> ppIndent 2 ++ "decl_" ++ ppMeth "SendEn" (s, i) ++ " = " ++ ppMeth "SendEn" (s, i) ++ ";\n") (tag sends)
-  ++ concatMap (\(i, (s, (Build_Mem n k p _))) -> condMem n k p $ ppIndent 2 ++ "decl_" ++ ppMem "Rq" (s, i) ++ " = " ++ ppMem "Rq" (s, i) ++ ";\n") (tag mems)
-  ++ concatMap (\(i, (s, (Build_Mem n k p _))) -> condMem n k p $ ppIndent 2 ++ "decl_" ++ ppMem "RqEn" (s, i) ++ " = " ++ ppMem "RqEn" (s, i) ++ ";\n") (tag mems)
-  ++ concatMap (\(i, (s, (Build_Mem n k p _))) -> condMem n k p $ ppIndent 2 ++ "decl_" ++ ppMem "WrIdx" (s, i) ++ " = " ++ ppMem "WrIdx" (s, i) ++ ";\n") (tag mems)
-  ++ concatMap (\(i, (s, (Build_Mem n k p _))) -> condMem n k p $ ppIndent 2 ++ "decl_" ++ ppMem "WrVal" (s, i) ++ " = " ++ ppMem "WrVal" (s, i) ++ ";\n") (tag mems)
-  ++ concatMap (\(i, (s, (Build_Mem n k p _))) -> condMem n k p $ ppIndent 2 ++ "decl_" ++ ppMem "WrEn" (s, i) ++ " = " ++ ppMem "WrEn" (s, i) ++ ";\n") (tag mems)
-  ++ concatMap (\(i, (s, (Build_MemU n k p))) -> condMem n k p $ ppIndent 2 ++ "decl_" ++ ppMem "URq" (s, i) ++ " = " ++ ppMem "URq" (s, i) ++ ";\n") (tag memUs)
-  ++ concatMap (\(i, (s, (Build_MemU n k p))) -> condMem n k p $ ppIndent 2 ++ "decl_" ++ ppMem "URqEn" (s, i) ++ " = " ++ ppMem "URqEn" (s, i) ++ ";\n") (tag memUs)
-  ++ concatMap (\(i, (s, (Build_MemU n k p))) -> condMem n k p $ ppIndent 2 ++ "decl_" ++ ppMem "UWrIdx" (s, i) ++ " = " ++ ppMem "UWrIdx" (s, i) ++ ";\n") (tag memUs)
-  ++ concatMap (\(i, (s, (Build_MemU n k p))) -> condMem n k p $ ppIndent 2 ++ "decl_" ++ ppMem "UWrVal" (s, i) ++ " = " ++ ppMem "UWrVal" (s, i) ++ ";\n") (tag memUs)
-  ++ concatMap (\(i, (s, (Build_MemU n k p))) -> condMem n k p $ ppIndent 2 ++ "decl_" ++ ppMem "UWrEn" (s, i) ++ " = " ++ ppMem "UWrEn" (s, i) ++ ";\n") (tag memUs)
-  ++ ppIndent 1 ++ "end\n"
+modElems :: Tree ModElem -> [(Integer, (String, ModElem))]
+modElems tree =
+  filter (sizeElem . Prelude.snd . Prelude.snd)
+    (Prelude.map (\(i, (path, elem)) -> (i, (intercalate "_" (reverse path), elem)))
+      (tag (dfsModElems tree)))
+
+ppPorts :: String -> Bool -> Int -> [(Integer, (String, ModElem))] -> String
+ppPorts term showDir q elems = concatMap ppPort elems
+  where
+    dir s = if showDir then s else ""
+    ppPort (i, (s, ESend k)) =
+      ppIndent q ++ dir "output " ++ ppKindImmStart q k ++ "decl_" ++ ppMeth "Send" (s, i) ++ term ++ "\n"
+      ++ ppIndent q ++ dir "output " ++ ppKindImmStart q Bool ++ "decl_" ++ ppMeth "SendEn" (s, i) ++ term ++ "\n"
+    ppPort (i, (s, ERecv k)) =
+      ppIndent q ++ dir "input " ++ ppKindImmStart q k ++ " " ++ ppMeth "Recv" (s, i) ++ term ++ "\n"
+    ppPort _ = ""
+
+ppModElemDecls :: Int -> [(Integer, (String, ModElem))] -> String
+ppModElemDecls q elems = concatMap ppModElemDecl elems
+  where
+    ppModElemDecl (i, (s, EReg r)) =
+      ppKindDecl q (regKind r) ++ "decl_" ++ ppReg (s, i) ++ ";\n"
+    ppModElemDecl (i, (s, EMem m)) =
+      ppKindDecl q (Array (memPort m) (Bit (clog2 (memSize m)))) ++ "decl_" ++ ppMem "Rq" (s, i) ++ ";\n"
+      ++ ppKindDecl q (Array (memPort m) Bool) ++ "decl_" ++ ppMem "RqEn" (s, i) ++ ";\n"
+      ++ ppKindDecl q (Bit (clog2 (memSize m))) ++ "decl_" ++ ppMem "WrIdx" (s, i) ++ ";\n"
+      ++ ppKindDecl q (memKind m) ++ "decl_" ++ ppMem "WrVal" (s, i) ++ ";\n"
+      ++ ppKindDecl q Bool ++ "decl_" ++ ppMem "WrEn" (s, i) ++ ";\n"
+      ++ ppKindDecl q (Array (memPort m) (memKind m)) ++ ppMem "Rp" (s, i) ++ ";\n"
+    ppModElemDecl (i, (s, ESend _)) = ""
+    ppModElemDecl (i, (s, ERecv _)) = ""
+
+ppCTmpDecls :: Int -> [(String, Integer, Kind)] -> String
+ppCTmpDecls q tmps = concatMap ppCTmpDecl tmps
+  where
+    ppCTmpDecl (s, idx, k) = ppKindDecl q k ++ ppTmp (s, idx) ++ ";\n"
+
+ppShadowDecls :: Int -> [(Integer, (String, ModElem))] -> String
+ppShadowDecls q elems = concatMap ppShadowDecl elems
+  where
+    ppShadowDecl (i, (s, EReg r)) =
+      ppKindDecl q (regKind r) ++ ppReg (s, i) ++ ";\n"
+    ppShadowDecl (i, (s, ESend k)) =
+      ppKindDecl q k ++ ppMeth "Send" (s, i) ++ ";\n"
+      ++ ppKindDecl q Bool ++ ppMeth "SendEn" (s, i) ++ ";\n"
+    ppShadowDecl (i, (s, EMem m)) =
+      ppKindDecl q (Array (memPort m) (Bit (clog2 (memSize m)))) ++ ppMem "Rq" (s, i) ++ ";\n"
+      ++ ppKindDecl q (Array (memPort m) Bool) ++ ppMem "RqEn" (s, i) ++ ";\n"
+      ++ ppKindDecl q (Bit (clog2 (memSize m))) ++ ppMem "WrIdx" (s, i) ++ ";\n"
+      ++ ppKindDecl q (memKind m) ++ ppMem "WrVal" (s, i) ++ ";\n"
+      ++ ppKindDecl q Bool ++ ppMem "WrEn" (s, i) ++ ";\n"
+    ppShadowDecl (i, (s, ERecv k)) = ""
+
+ppRegisterResets :: Int -> String -> [(Integer, (String, ModElem))] -> String
+ppRegisterResets q op elems = concatMap ppRegisterReset elems
+  where
+    ppRegisterReset (i, (s, EReg (Build_Reg k (Just val)))) =
+      ppIndent q ++ "decl_" ++ ppReg (s, i) ++ " " ++ op ++ " " ++ ppConst k val ++ ";\n"
+    ppRegisterReset _ = ""
+
+ppCTmpInits :: Int -> [(String, Integer, Kind)] -> String
+ppCTmpInits q tmps = concatMap ppCTmpInit tmps
+  where
+    ppCTmpInit (s, idx, k) =
+      ppIndent q ++ ppTmp (s, idx) ++ " = " ++ show (size k) ++ "'h0;\n"
+
+ppShadowInits :: Int -> [(Integer, (String, ModElem))] -> String
+ppShadowInits q elems = concatMap ppShadowInit elems
+  where
+    ppShadowInit (i, (s, EReg r)) =
+      ppIndent q ++ ppReg (s, i) ++ " = decl_" ++ ppReg (s, i) ++ ";\n"
+    ppShadowInit (i, (s, ESend k)) =
+      ppIndent q ++ ppMeth "Send" (s, i) ++ " = " ++ show (size k) ++ "'h0;\n"
+      ++ ppIndent q ++ ppMeth "SendEn" (s, i) ++ " = 1'b0;\n"
+    ppShadowInit (i, (s, EMem m)) =
+      ppIndent q ++ ppMem "Rq" (s, i) ++ " = " ++ show (memPort m * clog2 (memSize m)) ++ "'h0;\n"
+      ++ ppIndent q ++ ppMem "RqEn" (s, i) ++ " = " ++ show (memPort m) ++ "'h0;\n"
+      ++ ppIndent q ++ ppMem "WrIdx" (s, i) ++ " = " ++ show (clog2 (memSize m)) ++ "'h0;\n"
+      ++ ppIndent q ++ ppMem "WrVal" (s, i) ++ " = " ++ show (size (memKind m)) ++ "'h0;\n"
+      ++ ppIndent q ++ ppMem "WrEn" (s, i) ++ " = 1'h0;\n"
+    ppShadowInit (i, (s, ERecv k)) = ""
+
+ppFinalAssigns :: Int -> [(Integer, (String, ModElem))] -> String
+ppFinalAssigns q elems = concatMap ppFinalAssign elems
+  where
+    ppFinalAssign (i, (s, ESend k)) =
+      ppIndent q ++ "decl_" ++ ppMeth "Send" (s, i) ++ " = " ++ ppMeth "Send" (s, i) ++ ";\n"
+      ++ ppIndent q ++ "decl_" ++ ppMeth "SendEn" (s, i) ++ " = " ++ ppMeth "SendEn" (s, i) ++ ";\n"
+    ppFinalAssign (i, (s, EMem m)) =
+      ppIndent q ++ "decl_" ++ ppMem "Rq" (s, i) ++ " = " ++ ppMem "Rq" (s, i) ++ ";\n"
+      ++ ppIndent q ++ "decl_" ++ ppMem "RqEn" (s, i) ++ " = " ++ ppMem "RqEn" (s, i) ++ ";\n"
+      ++ ppIndent q ++ "decl_" ++ ppMem "WrIdx" (s, i) ++ " = " ++ ppMem "WrIdx" (s, i) ++ ";\n"
+      ++ ppIndent q ++ "decl_" ++ ppMem "WrVal" (s, i) ++ " = " ++ ppMem "WrVal" (s, i) ++ ";\n"
+      ++ ppIndent q ++ "decl_" ++ ppMem "WrEn" (s, i) ++ " = " ++ ppMem "WrEn" (s, i) ++ ";\n"
+    ppFinalAssign (i, (s, EReg _)) = ""
+    ppFinalAssign (i, (s, ERecv _)) = ""
+
+ppRegisterUpdates :: Int -> [(Integer, (String, ModElem))] -> String
+ppRegisterUpdates q elems = concatMap ppRegisterUpdate elems
+  where
+    ppRegisterUpdate (i, (s, EReg r)) =
+      ppIndent q ++ "decl_" ++ ppReg (s, i) ++ " <= " ++ ppReg (s, i) ++ ";\n"
+    ppRegisterUpdate (i, (s, ESend _)) = ""
+    ppRegisterUpdate (i, (s, EMem _)) = ""
+    ppRegisterUpdate (i, (s, ERecv _)) = ""
+
+ppModMemParams :: Int -> Mem -> String
+ppModMemParams q (Build_Mem n k p initVal) =
+  ppIndent q ++ ".n(" ++ show n ++ "),\n" ++
+  ppIndent q ++ ".clgn(" ++ show (clog2 n) ++ "),\n" ++
+  ppIndent q ++ ".sizeK(" ++ show (size k) ++ "),\n" ++
+  ppIndent q ++ ".p(" ++ show p ++ "),\n" ++
+  case initVal of
+    Just (Just val) ->
+      ppIndent q ++ ".init(1),\n" ++
+      ppIndent q ++ ".def(0),\n" ++
+      ppIndent q ++ ".initVal(" ++ ppConst (Array n k) val ++ ")\n"
+    Just Nothing ->
+      ppIndent q ++ ".init(1),\n" ++
+      ppIndent q ++ ".def(1)\n"
+    Nothing ->
+      ppIndent q ++ ".init(0)\n"
+
+ppModMemPorts :: Int -> (String, Integer) -> String
+ppModMemPorts q (s, i) =
+  ppIndent q ++ ".Rq(" ++ ("decl_" ++ ppMem "Rq" (s, i)) ++ "),\n" ++
+  ppIndent q ++ ".RqEn(" ++ ("decl_" ++ ppMem "RqEn" (s, i)) ++ "),\n" ++
+  ppIndent q ++ ".WrIdx(" ++ ("decl_" ++ ppMem "WrIdx" (s, i)) ++ "),\n" ++
+  ppIndent q ++ ".WrVal(" ++ ("decl_" ++ ppMem "WrVal" (s, i)) ++ "),\n" ++
+  ppIndent q ++ ".WrEn(" ++ ("decl_" ++ ppMem "WrEn" (s, i)) ++ "),\n" ++
+  ppIndent q ++ ".Rp(" ++ ppMem "Rp" (s, i) ++ "),\n" ++
+  ppIndent q ++ ".CLK(CLK),\n" ++
+  ppIndent q ++ ".RESET(RESET)\n"
+
+ppMemInstantiations :: Int -> [(Integer, (String, ModElem))] -> String
+ppMemInstantiations q elems = concatMap ppMemInst elems
+  where
+    ppMemInst (i, (s, EMem m)) =
+      ppIndent q ++ "verilog_mem#(\n" ++
+      ppModMemParams (q+1) m ++
+      ppIndent q ++ ") mem_" ++ ppMem "" (s, i) ++ " (\n" ++
+      ppModMemPorts (q+1) (s, i) ++
+      ppIndent q ++ ");\n"
+    ppMemInst _ = ""
+
+ppTopInstantiation :: Int -> [(Integer, (String, ModElem))] -> String
+ppTopInstantiation q elems =
+  ppIndent q ++ "top inst (\n"
+  ++ concatMap ppTopInstPort elems ++ "\n"
+  ++ ppIndent (q+1) ++ ".CLK(CLK),\n"
+  ++ ppIndent (q+1) ++ ".RESET(RESET)\n"
+  ++ ppIndent q ++ ");\n"
+  where
+    ppTopInstPort (i, (s, ESend k)) =
+      ppIndent (q+1) ++ ".decl_" ++ ppMeth "Send" (s, i) ++ "(decl_" ++ ppMeth "Send" (s, i) ++ "),\n"
+      ++ ppIndent (q+1) ++ ".decl_" ++ ppMeth "SendEn" (s, i) ++ "(decl_" ++ ppMeth "SendEn" (s, i) ++ "),\n"
+    ppTopInstPort (i, (s, ERecv k)) =
+      ppIndent (q+1) ++ "." ++ ppMeth "Recv" (s, i) ++ "(" ++ ppMeth "Recv" (s, i) ++ "),\n"
+    ppTopInstPort _ = ""
+
+ppTop :: CompiledModule -> String
+ppTop ((tree, tmpsRaw), code) =
+  "module top (\n"
+  ++ ppPorts "," True 1 elems ++ "\n"
+  ++ "  input CLK,\n"
+  ++ "  input RESET\n"
+  ++ ");\n"
+  ++ ppModElemDecls 1 elems ++ "\n"
+  ++ ppCTmpDecls 1 tmps ++ "\n"
+  ++ ppShadowDecls 1 elems ++ "\n"
+  ++ ppMemInstantiations 1 elems ++ "\n"
+  ++ "  initial begin\n"
+  ++ ppRegisterResets 2 "=" elems
+  ++ "  end\n\n"
+  ++ "  always_comb begin\n"
+  ++ ppCTmpInits 2 tmps ++ "\n"
+  ++ ppShadowInits 2 elems ++ "\n"
+  ++ ppCompiled 2 code ++ "\n"
+  ++ ppFinalAssigns 2 elems
+  ++ "  end\n\n"
+  ++ "  always_ff @(posedge CLK) begin\n"
+  ++ "    if (RESET) begin\n"
+  ++ ppRegisterResets 3 "<=" elems
+  ++ "    end else begin\n"
+  ++ ppRegisterUpdates 3 elems
+  ++ "    end\n"
+  ++ "  end\n"
+  ++ "endmodule\n\n"
+  ++ "module tb();\n"
+  ++ "  logic CLK;\n"
+  ++ "  logic RESET;\n\n"
+  ++ ppPorts ";" False 1 elems ++ "\n"
+  ++ ppTopInstantiation 1 elems ++ "\n"
+  ++ "  initial begin\n"
+  ++ "    CLK = 1'h0;\n"
+  ++ "    RESET = 1'h1;\n"
+  ++ "    RESET = #40 1'h0;\n"
+  ++ "    #2000 $finish;\n"
+  ++ "  end\n\n"
+  ++ "  always begin\n"
+  ++ "    CLK = #10 1'h1;\n"
+  ++ "    CLK = #10 1'h0;\n"
+  ++ "  end\n"
   ++ "endmodule\n"
+  where
+    elems = modElems tree
+    len = genericLength tmpsRaw
+    tmpsOriginal = Prelude.map (\(i, (s, k)) -> (s, len - 1 - i, k)) (tag tmpsRaw)
+    tmps = filter (\(_, _, k) -> size k > 0) tmpsOriginal
