Theorems.v
@@ -4,108 +4,69 @@ Require Import Guru.Library Guru.Syntax Guru.Semantics.
 Set Implicit Arguments.
 Set Asymmetric Patterns.
 
+
+
 Section InversionSemAction.
-  Variable modLists: ModLists.
+  Variable t: Tree ModElem.
 
   Theorem InversionSemAction
-    k (a: Action type modLists k) old new puts gets ret
-    (semA: SemAction a old new puts gets ret):
+    k (a: @Action type t k) old new ret
+    (semA: SemAction a old new ret):
     match a with
-    | ReadReg s x cont => SemAction (cont (readDiffTuple old.(stateRegs) x)) old new puts gets ret
+    | ReadReg s x cont => SemAction (cont (castStateReg x (readTreeState t old x.(regPath)))) old new ret
     | WriteReg x v cont =>
-        SemAction cont {|stateRegs := updDiffTuple old.(stateRegs) (evalExpr v);
-                         stateMems := old.(stateMems);
-                         stateRegUs := old.(stateRegUs);
-                         stateMemUs := old.(stateMemUs)|} new puts gets ret
+        SemAction cont (writeTreeState t old x.(regPath) (castStateRegInv x (evalExpr v))) new ret
     | ReadRqMem x i p cont =>
         SemAction
           cont
-          {|stateRegs := old.(stateRegs);
-            stateMems := let arr := readDiffTuple old.(stateMems) x in
-                         updDiffTuple (old.(stateMems))
-                           (fst arr, updSameTuple (snd arr) p (readNatToFinType (Default _) (readSameTuple (fst arr))
-                                                                 (Z.to_nat (Zmod.to_Z (evalExpr i)))));
-            stateRegUs := old.(stateRegUs);
-            stateMemUs := old.(stateMemUs)|} new puts gets ret
+          (let arr := castStateMem x (readTreeState t old x.(memPath)) in
+           let val := nth (Z.to_nat (Zmod.to_Z (evalExpr i))) arr.(Fst).(tupleElems) (Default _) in
+           writeTreeState t old x.(memPath) (castStateMemInv x (arr.(Fst) ,, updSameTuple arr.(Snd) p val))) new ret
     | ReadRpMem s x p cont =>
-        SemAction (cont (readSameTuple (snd (readDiffTuple old.(stateMems) x)) p)) old new puts gets ret
+        SemAction (cont (readSameTuple (castStateMem x (readTreeState t old x.(memPath))).(Snd) p)) old new ret
     | WriteMem x i v cont =>
         SemAction
           cont
-          {|stateRegs := old.(stateRegs);
-            stateMems := let arr := readDiffTuple old.(stateMems) x in
-                         updDiffTuple (old.(stateMems))
-                           (updSameTupleNat (fst arr) (Z.to_nat (Zmod.to_Z (@evalExpr _ i))) (evalExpr v), snd arr);
-            stateRegUs := old.(stateRegUs);
-            stateMemUs := old.(stateMemUs)|} new puts gets ret
-    | ReadRegU s x cont => SemAction (cont (readDiffTuple old.(stateRegUs) x)) old new puts gets ret
-    | WriteRegU x v cont =>
-        SemAction cont {|stateRegs := old.(stateRegs);
-                         stateMems := old.(stateMems);
-                         stateRegUs := updDiffTuple old.(stateRegUs) (evalExpr v);
-                         stateMemUs := stateMemUs old|} new puts gets ret
-    | ReadRqMemU x i p cont =>
-        SemAction
-          cont
-          {|stateRegs := old.(stateRegs);
-            stateMems := old.(stateMems);
-            stateRegUs := old.(stateRegUs);
-            stateMemUs := let arr := readDiffTuple old.(stateMemUs) x in
-                          updDiffTuple (old.(stateMemUs))
-                            (fst arr, updSameTuple (snd arr) p (readNatToFinType (Default _) (readSameTuple (fst arr))
-                                                                  (Z.to_nat (Zmod.to_Z (evalExpr i)))))|}
-          new puts gets ret
-    | ReadRpMemU s x p cont =>
-        SemAction (cont (readSameTuple (snd (readDiffTuple old.(stateMemUs) x)) p)) old new puts gets ret
-    | WriteMemU x i v cont =>
-        SemAction
-          cont
-          {|stateRegs := old.(stateRegs);
-            stateMems := old.(stateMems);
-            stateRegUs := old.(stateRegUs);
-            stateMemUs := let arr := readDiffTuple old.(stateMemUs) x in
-                          updDiffTuple (old.(stateMemUs))
-                            (updSameTupleNat (fst arr) (Z.to_nat (Zmod.to_Z (@evalExpr _ i))) (evalExpr v), snd arr)|}
-          new puts gets ret
+          (let arr := castStateMem x (readTreeState t old x.(memPath)) in
+           writeTreeState t old x.(memPath) (castStateMemInv x (updSameTupleNat arr.(Fst) (Z.to_nat (Zmod.to_Z (evalExpr i))) (evalExpr v) ,, arr.(Snd)))) new ret
     | Send x v cont =>
-        exists putsStep,
-        SemAction cont old new putsStep gets ret /\
-          puts = updDiffTuple putsStep (evalExpr v :: readDiffTuple putsStep x)
+        SemAction cont
+          (let currentTrace := castStateSend x (readTreeState t old x.(sendPath)) in
+           writeTreeState t old x.(sendPath) (castStateSendInv x (evalExpr v :: currentTrace)))
+          new ret
     | Recv s x cont =>
-        exists recvStep getsStep,
-        SemAction (cont recvStep) old new puts getsStep ret /\
-          gets = updDiffTuple getsStep (recvStep :: readDiffTuple getsStep x)
+        exists recvVal,
+        SemAction (cont recvVal)
+          (let currentTrace := castStateRecv x (readTreeState t old x.(recvPath)) in
+           writeTreeState t old x.(recvPath) (castStateRecvInv x (recvVal :: currentTrace)))
+          new ret
     | LetExp s k' e cont =>
-        SemAction (cont (evalExpr e)) old new puts gets ret
-    | LetAction s k' a cont =>
-        exists newStep putsStep getsStep retStep interPuts interGets,
-        SemAction a old newStep putsStep getsStep retStep /\
-          SemAction (cont retStep) newStep new interPuts interGets ret /\
-          (puts = combineDiffTuple (fun _ => @List.app _) putsStep interPuts) /\
-          gets = combineDiffTuple (fun _ => @List.app _) getsStep interGets
+        SemAction (cont (evalExpr e)) old new ret
+    | LetAction s k' a' cont =>
+        exists newStep retStep,
+        SemAction a' old newStep retStep /\
+          SemAction (cont retStep) newStep new ret
     | NonDet s k' cont =>
         exists v,
-        SemAction (cont v) old new puts gets ret
-    | IfElse s p k' t f cont =>
-        exists newStep putsStep getsStep retStep interPuts interGets,
-        (evalExpr p = true -> SemAction t old newStep putsStep getsStep retStep) /\
-          (evalExpr p = false -> SemAction f old newStep putsStep getsStep retStep) /\
-          SemAction (cont retStep) newStep new interPuts interGets ret /\
-          (puts = combineDiffTuple (fun _ => @List.app _) putsStep interPuts) /\
-          gets = combineDiffTuple (fun _ => @List.app _) getsStep interGets
+        SemAction (cont v) old new ret
+    | IfElse s p k' t_branch f_branch cont =>
+        exists newStep retStep,
+        (evalExpr p = true -> SemAction t_branch old newStep retStep) /\
+          (evalExpr p = false -> SemAction f_branch old newStep retStep) /\
+          SemAction (cont retStep) newStep new ret
     | System ls cont =>
-        SemAction cont old new puts gets ret
+        SemAction cont old new ret
     | Return e =>
-        new = old /\ (puts = defaultDiffTuple (fun _ => nil) _) /\ (gets = defaultDiffTuple (fun _ => nil) _) /\
-          ret = evalExpr e
+        new = old /\ ret = evalExpr e
     end.
   Proof.
     destruct semA; eauto; repeat eexists; eauto; try discriminate.
   Qed.
 End InversionSemAction.
 
+
 Section LetExpr.
-  Variable modLists: ModLists.
+  Variable t: Tree ModElem.
 
   Local Ltac destructAll := repeat (match goal with
                                     | H: exists _, _ |- _ => destruct H
@@ -113,195 +74,193 @@ Section LetExpr.
                                     end).
 
   Theorem SemActionLetExpr k (le: LetExpr type k):
-    forall old new puts gets ret,
-      SemAction (@toAction _ modLists _ le) old new puts gets ret ->
-      new = old /\ (puts = defaultDiffTuple (fun _ => nil) _) /\ (gets = defaultDiffTuple (fun _ => nil) _) /\
-        ret = (evalLetExpr le).
+    forall old new ret,
+      SemAction (@toAction _ t _ le) old new ret ->
+      new = old /\ ret = (evalLetExpr le).
   Proof.
     induction le; simpl; intros;
       match goal with
-      | H: SemAction _ _ _ _ _ _ |- _ => apply InversionSemAction in H
+      | H: SemAction _ _ _ _ |- _ => apply InversionSemAction in H
       end; auto.
     - destructAll.
-      specialize (IHle _ _ _ _ _ H0).
-      specialize (H _ _ _ _ _ _ H1).
+      specialize (IHle _ _ _ H0).
+      specialize (H _ _ _ _ H1).
       destructAll; subst; simpl.
-      repeat split; auto; apply combineDiffTupleDef; auto.
+      auto.
     - destructAll.
       case_eq (evalExpr p); intros sth.
-      + specialize (IHle1 _ _ _ _ _ (H0 sth)).
-        specialize (H _ _ _ _ _ _ H2).
-        destructAll; subst; simpl.
-        repeat split; auto; apply combineDiffTupleDef; auto.
-      + specialize (IHle2 _ _ _ _ _ (H1 sth)).
-        specialize (H _ _ _ _ _ _ H2).
-        destructAll; subst; simpl.
-        repeat split; auto; apply combineDiffTupleDef; auto.
+      + specialize (IHle1 _ _ _ (H0 sth)).
+        specialize (H _ _ _ _ H2).
+        destructAll; subst; simpl; auto.
+      + specialize (IHle2 _ _ _ (H1 sth)).
+        specialize (H _ _ _ _ H2).
+        destructAll; subst; simpl; auto.
   Qed.
 End LetExpr.
 
-Unset Strict Implicit.
-Section mapDiffTuple_createDiffTupleMap.
-  Variable A B: Type.
-  Variable Conv1: A -> Type.
-  Variable Conv2: A -> Type.
-  Variable f: forall a, Conv1 a -> Conv2 a.
-  Variable mapF: B -> A.
-  Variable g: forall b, Conv1 (mapF b).
-  Theorem mapDiffTuple_createDiffTupleMap ls:
-    (mapDiffTuple f (createDiffTupleMap (mapF := mapF) g ls)) =
-      createDiffTupleMap (mapF := mapF) (fun a => f (g a)) ls.
-  Proof.
-    induction ls; simpl; auto.
-    rewrite IHls.
-    auto.
-  Qed.
-End mapDiffTuple_createDiffTupleMap.
-Set Strict Implicit.
+Theorem Zmod_1_0: forall x: Zmod 1, x = Zmod.zero.
+Proof.
+  intros.
+  apply (Zmod.hprop_Zmod_1 x Zmod.zero).
+Qed.
 
-Section ExistsInitModConsistent.
-  Theorem ExistsInitModConsistent (decl: ModDecl): exists state, @InitModConsistent decl state.
-  Proof.
-    eexists.
-    eexact (@InitModStateCreate decl _
-              (defaultDiffTuple (fun x => Default (snd x)) decl.(modRegUs))
-              (defaultDiffTuple (fun x => (Default (Array (snd x).(memUSize) (snd x).(memUKind)),
-                                            Default (Array (snd x).(memUPort) (snd x).(memUKind))))
-                 decl.(modMemUs))
-              (mapDiffTuple_createDiffTupleMap
-                 (Conv1 := fun x => (type (Array (snd x).(memUSize) (snd x).(memUKind)) *
-                                       type (Array (snd x).(memUPort) (snd x).(memUKind)))%type)
-                 (fun _ => fst)
-                 (mapF := fun x => (fst x, memToMemU (snd x)))
-                 (fun x => (memInitFull (snd x), Default (Array (snd x).(memPort) (snd x).(memKind))))
-                 decl.(modMems))
-              _
-              eq_refl).
-  Qed.
-End ExistsInitModConsistent.
+
+Definition InitStateElemConsistentPf (e: ModElem) : InitStateElemConsistent e (InitStateElem e) :=
+  match e return InitStateElemConsistent e (InitStateElem e) with
+  | EReg r =>
+      match r.(regInit) as opt return
+        (match opt with
+         | None => fun s => True
+         | Some init => fun s => s = init
+         end)
+        (match opt with
+         | None => Default (regKind r)
+         | Some init => init
+         end)
+      with
+      | None => I
+      | Some init => eq_refl
+      end
+  | EMem m =>
+      match m.(memInit) as opt return
+        (match opt with
+         | None => fun s => True
+         | Some _ => fun s => s.(Fst) = memInitFull m
+         end) (memInitFull m ,, Default (Array m.(memPort) m.(memKind)))
+      with
+      | None => I
+      | Some _ => eq_refl
+      end
+  | ESend _ => eq_refl
+  | ERecv _ => eq_refl
+  end.
+
+Fixpoint InitStateConsistentPf (t: Tree ModElem) : InitStateConsistent t (InitState t) :=
+  match t return InitStateConsistent t (InitState t) with
+  | Leaf name a => InitStateElemConsistentPf a
+  | Node name children =>
+      (fix loop (ls: list (Tree ModElem)) :
+         (fix loop (ls : list (Tree ModElem)) : ModListTreeState ls -> Prop :=
+            match ls with
+            | nil => fun _ => True
+            | x :: xs => fun s => InitStateConsistent x s.(Fst) /\ loop xs s.(Snd)
+            end) ls
+           ((fix loop (ls : list (Tree ModElem)) : ModListTreeState ls :=
+              match ls with
+              | nil => tt
+              | x :: xs => (InitState x ,, loop xs)
+              end) ls) :=
+         match ls return
+           (fix loop (ls : list (Tree ModElem)) : ModListTreeState ls -> Prop :=
+              match ls with
+              | nil => fun _ => True
+              | x :: xs => fun s => InitStateConsistent x s.(Fst) /\ loop xs s.(Snd)
+              end) ls
+             ((fix loop (ls : list (Tree ModElem)) : ModListTreeState ls :=
+                match ls with
+                | nil => tt
+                | x :: xs => (InitState x ,, loop xs)
+                end) ls)
+         with
+         | nil => I
+         | x :: xs => conj (InitStateConsistentPf x) (loop xs)
+         end) children
+  end.
+
+Definition ExistsInitModConsistent (t: Tree ModElem) : exists old, InitStateConsistent t old.
+Proof.
+  exists (InitState t).
+  apply InitStateConsistentPf.
+Qed.
 
 Section StepInclusion.
-  Variable m1 m2: Mod.
-  Variable rel: ModStateModDecl (modDecl m1) -> ModStateModDecl (modDecl m2) -> Prop.
-  Variable initRel: forall init1, InitModConsistent init1 ->
-                                  forall init2, InitModConsistent init2 -> rel init1 init2.
-  Variable sameSends: modSends (modDecl m1) = modSends (modDecl m2).
-  Variable sameRecvs: modRecvs (modDecl m1) = modRecvs (modDecl m2).
+  Variable t1 t2: Tree ModElem.
+  Variable m1: Mod t1.
+  Variable m2: Mod t2.
+  Variable rel: TreeState ModElemState t1 -> TreeState ModElemState t2 -> Prop.
+  Variable relConsistent: forall old1 old2,
+      InitStateConsistent t1 old1 ->
+      rel old1 old2 ->
+      InitStateConsistent t2 old2.
 
-  Variable step: forall a1 (old1 new1: ModStateModDecl (modDecl m1)) puts gets,
-      In a1 (modActions m1 type) ->
-      SemAction a1 old1 new1 puts gets Zmod.zero ->
-      forall old2: ModStateModDecl (modDecl m2),
+  Variable stepMod: forall a1 old1 new1,
+      In a1 (m1 type) ->
+      SemAction a1 old1 new1 Zmod.zero ->
+      forall old2: TreeState ModElemState t2,
         rel old1 old2 ->
-        exists (a2: Action _ _ (Bit 0)) (new2: ModStateModDecl (modDecl m2)),
-          In a2 (modActions m2 type) /\ rel new1 new2 /\
-          SemAction a2 old2 new2
-            (match sameSends in _ = Y return _ Y with
-             | eq_refl => puts
-             end)
-            (match sameRecvs in _ = Y return _ Y with
-             | eq_refl => gets
-             end) Zmod.zero.
+        exists a2 new2,
+          In a2 (m2 type) /\ SemAction a2 old2 new2 Zmod.zero /\
+          rel new1 new2.
 
-  Lemma stepInclusionHelper: forall (old1 new1: ModStateModDecl (modDecl m1)) puts gets,
-      SemAnyAction (modActions m1 type) old1 new1 puts gets ->
-      forall old2: ModStateModDecl (modDecl m2),
-        rel old1 old2 ->
-        exists (new2: ModStateModDecl (modDecl m2)),
-          rel new1 new2 /\ SemAnyAction (modActions m2 type) old2 new2
-                             (match sameSends in _ = Y return _ Y with
-                              | eq_refl => puts
-                              end)
-                             (match sameRecvs in _ = Y return _ Y with
-                              | eq_refl => gets
-                              end).
+  Lemma stepInclusionHelper: forall s1 s2,
+      SemAnyAction (m1 type) s1 s2 ->
+      forall old2,
+        rel s1 old2 ->
+        exists new2,
+          rel s2 new2 /\
+          SemAnyAction (m2 type) old2 new2.
   Proof.
-    unfold getModLists in *; unfold SemAnyAction; induction 1; intros; subst; simpl in *.
-    - exists old2.
-      split; [intuition|].
-      constructor 1; auto; clear - sameSends sameRecvs.
-      + destruct sameSends; auto.
-      + destruct sameRecvs; auto.
-    - destruct step0.
-      specialize (@step a old newStep putsStep getsStep inA aPf old2 H0) as
-        [a2 [newStep2 [inA2 [relNewStep2 semA2]]]].
-      specialize (IHMultiStep newStep2 relNewStep2) as [new2 [relNew2 rest]].
+    induction 1 as [old_nil new_nil eqPf | old_cons new_cons newStep step rest IHrest]; intros.
+    - subst.
+      exists old2.
+      split; [exact H | constructor 1; auto].
+    - destruct step.
+      specialize (@stepMod a old newStep inA aPf old2 H) as H_step.
+      destruct H_step as [a2 [newStep2 [inA2 [semA2 relNewStep2]]]].
+      specialize (IHrest newStep2 relNewStep2) as [new2 [relNew2 restSteps]].
       exists new2.
-      split; [intuition|].
-      constructor 2 with (puts := match sameSends in (_ = Y) return (FuncIo Y) with
-                                  | eq_refl => puts
-                                  end)
-                         (gets := match sameRecvs in (_ = Y) return (FuncIo Y) with
-                                  | eq_refl => gets
-                                  end)
-                         (newStep := newStep2)
-                         (putsStep := match sameSends in (_ = Y) return (FuncIo Y) with
-                                      | eq_refl => putsStep
-                                      end)
-                         (getsStep := match sameRecvs in (_ = Y) return (FuncIo Y) with
-                                      | eq_refl => getsStep
-                                      end); auto; try (constructor 1 with (a := a2); auto);
-        clear - sameSends sameRecvs.
-      + destruct sameSends; auto.
-      + destruct sameRecvs; auto.
+      split; [exact relNew2 |].
+      econstructor 2; eauto.
+      constructor 1 with (a := a2); auto.
   Qed.
 
-  Theorem StepInclusion: TraceInclusion m1 m2.
+  Theorem StepInclusion: TraceInclusion m1 m2 rel.
   Proof.
-    constructor 1 with (traceSendsEq := sameSends) (traceRecvsEq := sameRecvs).
-    intros.
-    destruct H as [old1 new1 old1Consistent semAny1].
-    pose proof (ExistsInitModConsistent (modDecl m2)) as [old2 old2Consistent].
-    specialize (initRel old1Consistent old2Consistent).
-    pose proof (stepInclusionHelper semAny1 initRel) as [new2 [new2Rel semAny2]].
-    eexists; eauto.
+    intros old1 new1 H_sem old2 relOld.
+    destruct H_sem as [old1 new1 old1Consistent semAny1].
+    pose proof (@relConsistent old1 old2 old1Consistent relOld) as old2Consistent.
+    pose proof (stepInclusionHelper semAny1 relOld) as [new2 [relNew2 semAny2]].
+    exists new2.
+    split.
+    - constructor; auto.
+    - exact relNew2.
   Qed.
 End StepInclusion.
 
 Section CombineActionsHelpers.
-  Variable modLists: ModLists.
+  Variable t: Tree ModElem.
 
-  Definition combineActionsType := @combineActions type.
-
-  Lemma addStep ls old new puts gets:
-    Step ls old new puts gets ->
-    forall (act: Action type modLists (Bit 0)),
-      Step (act :: ls) old new puts gets.
+  Lemma addStep ls old new:
+    Step ls old new ->
+    forall (act: @Action type t (Bit 0)),
+      Step (act :: ls) old new.
   Proof.
     intros.
     destruct H; subst.
     constructor 1 with (a := a); simpl; tauto.
   Qed.
 
-  Lemma addSemAnyAction ls old new puts gets:
-    SemAnyAction ls old new puts gets ->
-    forall (a: Action type modLists (Bit 0)),
-      SemAnyAction (a :: ls) old new puts gets.
+  Lemma addSemAnyAction ls old new:
+    SemAnyAction ls old new ->
+    forall (a: @Action type t (Bit 0)),
+      SemAnyAction (a :: ls) old new.
   Proof.
-    unfold SemAnyAction.
     induction 1; subst; intros.
     - constructor 1; auto.
     - econstructor 2 with (newStep := newStep); eauto.
       apply addStep; auto.
   Qed.
 
-  Theorem Zmod_1_0: forall x: Zmod 1, x = Zmod.zero.
+  Lemma combineSemActionToSemAnyAction (ls: list (@Action type t (Bit 0))):
+    forall old new,
+      SemAction (combineActions ls) old new Zmod.zero ->
+      SemAnyAction ls old new.
   Proof.
-    intros.
-    apply (Zmod.hprop_Zmod_1 x Zmod.zero).
-  Qed.
-
-  Lemma combineSemActionToSemAnyAction (ls: list (Action type modLists (Bit 0))):
-    forall old new puts gets,
-      SemAction (combineActionsType ls) old new puts gets Zmod.zero ->
-      SemAnyAction ls old new puts gets.
-  Proof.
-    induction ls; simpl; intros; apply InversionSemAction in H.
-    - destruct H as [? [? [? ?]]]; subst.
+    induction ls; simpl; intros; apply InversionSemAction in H; cbn in H.
+    - destruct H; subst.
       constructor 1; auto.
-    - destruct H as
-        [newStep [putsStep [getsStep [retStep [interPuts [interGets [semA [semCb [putsEq getsEq]]]]]]]]].
-      specialize (IHls _ _ _ _ semCb).
+    - destruct H as [newStep [retStep [semA semCb]]].
+      specialize (IHls _ _ semCb).
       pose proof (Zmod.hprop_Zmod_1 retStep Zmod.zero) as retEq.
       subst.
       pose proof (addSemAnyAction IHls a) as pf.
@@ -311,28 +270,26 @@ Section CombineActionsHelpers.
   Qed.
 
   Section CombineSemAnyAction.
-    Variable ls: list (Action type modLists (Bit 0)).
+    Variable ls: list (@Action type t (Bit 0)).
     Lemma combineSemAnyActions:
-      forall old new1 puts1 gets1 new2 puts2 gets2,
-        SemAnyAction ls old new1 puts1 gets1 ->
-        SemAnyAction ls new1 new2 puts2 gets2 ->
-        SemAnyAction ls old new2 (combineDiffTuple (fun _ => @List.app _) puts1 puts2)
-          (combineDiffTuple (fun _ => @List.app _) gets1 gets2).
+      forall old new1 new2,
+        SemAnyAction ls old new1 ->
+        SemAnyAction ls new1 new2 ->
+        SemAnyAction ls old new2.
     Proof.
-      induction 1; subst; simpl; intros.
-      - repeat (rewrite combineDiffTupleDef; auto).
-      - specialize (IHMultiStep H0).
-        repeat (erewrite <- combineDiffTupleAssoc by (intros; eapply app_assoc; eauto)).
-        econstructor 2; eauto.
+      induction 1 as [old_nil new_nil eqPf | old_cons new_cons newStep step rest IHrest]; intros.
+      - subst.
+        exact H.
+      - econstructor 2 with (newStep := newStep); eauto.
     Qed.
   End CombineSemAnyAction.
 
-  Lemma combineActionsSemantics (ls: list (Action type modLists (Bit 0))):
-    forall old new puts gets,
-      SemAnyAction (combineActionsType ls :: nil) old new puts gets ->
-      SemAnyAction ls old new puts gets.
+  Lemma combineActionsSemantics (ls: list (@Action type t (Bit 0))):
+    forall old new,
+      SemAnyAction (combineActions ls :: nil) old new ->
+      SemAnyAction ls old new.
   Proof.
-    induction 1.
+    induction 1 as [old_nil new_nil eqPf | old_cons new_cons newStep step rest IHrest]; intros.
     - constructor 1; subst; auto.
     - subst.
       destruct step.
@@ -343,21 +300,20 @@ Section CombineActionsHelpers.
 End CombineActionsHelpers.
 
 Section CombineActionsTraceInclusion.
-  Variable decl: ModDecl.
-  Variable ls: forall ty,
-      list (Action ty (getModLists decl) (Bit 0)).
+  Variable t: Tree ModElem.
+  Variable ls: forall ty, list (@Action ty t (Bit 0)).
 
-  Theorem CombineActionsTraceInclusion: TraceInclusion {|modDecl := decl;
-                                                         modActions := fun ty => combineActions (ls ty) :: nil |}
-                                                       {|modDecl := decl;
-                                                         modActions := ls |}.
+  Theorem CombineActionsTraceInclusion: TraceInclusion (fun ty => combineActions (ls ty) :: nil)
+                                                              ls
+                                                              (fun s1 s2 => s1 = s2).
   Proof.
-    econstructor 1 with
-      (m1 := {| modDecl := decl; modActions := fun ty => combineActions (ls ty) :: nil |})
-      (m2 := {| modDecl := decl; modActions := ls |})
-      (traceSendsEq := eq_refl) (traceRecvsEq := eq_refl); auto; simpl; intros.
-    destruct H.
-    apply combineActionsSemantics in steps.
-    econstructor; eauto.
+    intros old1 new1 H_sem old2 relOld.
+    destruct H_sem as [old1 new1 old1Consistent semAny1].
+    subst old2.
+    apply combineActionsSemantics in semAny1.
+    exists new1.
+    split.
+    - constructor; auto.
+    - reflexivity.
   Qed.
 End CombineActionsTraceInclusion.
