Ltacs.v
@@ -1,29 +1,52 @@
 From Stdlib Require Import String List ZArith Zmod.
 Require Import Guru.Library Guru.Syntax Guru.Semantics Guru.Theorems Guru.Notations.
 
-Ltac simplifyInit :=
+Ltac simplifyHyps stateRel :=
   repeat match goal with
-    | H: InitModConsistent _ |- _ => destruct H
-    | t: unit |- _ => destruct t
-    end; simpl in *; subst;
-  constructor; unfold readDiffTupleStr; auto; intros; try discriminate.
+    | H: stateRel _ _ |- _ => destruct H
+    | H: InitStateConsistent _ _ |- _ => simpl in H
+    | H: TreeState ModElemState (Leaf _ _) |- _ => simpl in H
+    | H: TreeState ModElemState _ |- _ => destruct H
+    | H: _ ** _ |- _ => destruct H
+    | H: exists _, _ |- _ => destruct H
+    | H: unit |- _ => clear H
+    | H: _ /\ _ |- _ => destruct H
+    end;
+  simpl in *;
+  repeat (
+    match goal with
+    | H: @Build_Prod _ _ ?x ?y = @Build_Prod _ _ ?a ?b |- _ =>
+        injection H; clear H; intros
+    end;
+    subst
+  );
+  subst.
 
-Ltac invertSemAction :=
+Ltac simulateStep specAction :=
+  exists specAction;
+  eexists;
+  split; [simpl; auto | split; [ repeat econstructor; eauto | constructor; simpl; auto ]].
+
+Ltac simulateRetv t :=
+  simulateStep (@Return type t (Bit 0) ConstDef).
+
+Ltac invertAction :=
   repeat match goal with
-    | H: @SemAction _ _ _ _ _ _ _ _ |- _ => apply InversionSemAction in H
+    | H: SemAction _ _ _ _ |- _ => apply InversionSemAction in H
     | H: exists _, _ |- _ => destruct H
     | H: _ /\ _ |- _ => destruct H
-    | H: context [evalExpr (Not _)] |- _ => simpl in H
-    | H: ?P = true -> @SemAction _ _ _ _ _ _ _ _ |- _ => destruct P eqn:?
+    | H: ?P = true -> SemAction _ _ _ _ |- _ => destruct P eqn:?
+    | H: ?P = false -> SemAction _ _ _ _ |- _ => destruct P eqn:?
     | H: ?a = ?a -> _ |- _ => specialize (H eq_refl)
     | H: true = false -> _ |- _ => clear H
     | H: false = true -> _ |- _ => clear H
-    end; subst; simpl.
+    end.
 
-Ltac useOld old := exists Retv, old;
-                                split; [auto| split; [|econstructor; eauto; simpl]];
-                                repeat match goal with
-                                  | H: Prod _ _ |- _ => destruct H
-                                  end; simpl in *;
-                                constructor; unfold readDiffTupleStr in *; simpl in *; subst; auto; intros;
-                                try discriminate.
+Ltac destructActionInList impl :=
+  unfold impl in *;
+  repeat match goal with
+    | H: In ?a _ |- _ =>
+        match type of a with
+        | @Action _ _ _ => destruct H; try discriminate; subst
+        end
+    end.
